LambdaLab.lean
@@ -85,3 +85,4 @@ import LambdaLab.Parser.Truncation.Mixfix
 import LambdaLab.Stlc.Named.Lang
 import LambdaLab.Stlc.Named.Mvars
 import LambdaLab.Stlc.Named.Solving
+import LambdaLab.Stlc.Named.Inference
